src/reflection.lean
@@ -4,7 +4,7 @@ Released under Apache 2.0 license as described in the file LICENSE.
 
 Authors: Jesse Han, Floris van Doorn
 -/
-import .fol .abel tactic.ring .completeness .zfc
+import .fol tactic.abel tactic.ring .completeness .zfc .abel
 
 open fol
 
@@ -52,7 +52,7 @@ by {simp}
 example : ∀ x y : ℤ, x + (y + y) = y + (y + x) :=
 by {tidy}
 
-def L_abel_structure_of_add_group (α : Type) [add_group α] : Structure L_abel :=
+def L_abel_structure_of_add_comm_group (α : Type) [add_comm_group α] : Structure L_abel :=
 begin
   refine ⟨α, λn f, _, λn r, by {cases r}⟩,
   {induction f, intro xs, exact 0,
@@ -60,9 +60,9 @@ begin
     exact (xs.nth 0 dec_trivial) + (xs.nth 1 dec_trivial)}
 end
 
-variables (α : Type) [add_group α]
+variables (α : Type) [add_comm_group α]
 
-local notation `α'` := L_abel_structure_of_add_group α
+local notation `α'` := L_abel_structure_of_add_comm_group α
 
 @[simp]lemma α'_α : ↥(α') = α := by refl
 
@@ -72,29 +72,35 @@ local notation `α'` := L_abel_structure_of_add_group α
 
 @[reducible]instance nonempty_α' : nonempty α' := ⟨0⟩
 
+@[reducible]instance has_neg_α' : has_neg α' := ⟨λ x, (-x : α)⟩
+
 @[simp]lemma zero_is_zero : @realize_bounded_term L_abel α' _ [] _ zero [] = (0 : α) := by refl
 
 @[simp]lemma plus_is_plus_l : ∀ x y : α', realize_bounded_term ([x,y]) (&0 +' &1) [] = x + y := by {intros, refl}
 
 @[simp]lemma plus_is_plus_r : ∀ x y : α', realize_bounded_term ([x,y]) (&1 +' &0) [] = y + x := by {intros, refl}
 
-theorem add_group_is_abelian_group {α : Type} [add_group α] : T_ab ⊆ Th(L_abel_structure_of_add_group α) :=
+example {α} [add_comm_group α] {x y : α} : x + y = y + x := by simp
+
+theorem add_comm_group_is_abelian_group {α : Type} [add_comm_group α] : T_ab ⊆ Th(L_abel_structure_of_add_comm_group α) :=
 begin
   intros a H, repeat{cases H},
-  {intros x y, change x + y = y + x, simp[add_comm], sorry},
-  repeat{sorry}
-  -- {intros x H, dsimp at H, unfold realize_bounded_formula, have : ∃ y : ℤ, x + y = 0,
-  -- by {refine ⟨-x, _⟩, simp}, rcases this with ⟨y, hy⟩, apply H y, simp[hy], refl},
-  -- {intro x, change 0 + x = x, rw[zero_add]},
-  -- {intro x, change x + 0 = x, rw[add_zero]},
-  -- {intros x y z, change x + y + z = x + (y + z), rw[add_assoc]}
+  {intros x y, change x + y = y + x, simp},
+  {intro x,
+  simp only [realize_bounded_formula_ex, realize_bounded_formula,realize_bounded_formula_and],
+  use -x, change (x + -x = 0 ∧ -x + x = 0), simp},
+  {intro x, change 0 + x = x, simp},
+  {intro x, change x + 0 = x, simp},
+  {intros x y z, change x + y + z = x + (y + z), simp}
 end
 
 
 example : ∀ x y : α, x + (y + y) = y + (y + x) :=
-begin sorry
-  -- apply @by_reflection L_abel T_ab ℤ' (by apply_instance) (ℤ'_is_abelian_group) _ _ _ _,
-  -- exact ∀' ∀' (&1 +' (&0 +' &0) ≃ &0 +' (&0 +' &1)), {refl}, exact T_ab_proves_x_y_y
+begin
+  refine by_reflection (T_ab) (∀ x y, x + (y + y) = y + (y + x)) (∀' ∀' (&1 +' (&0 +' &0) ≃ &0 +' (&0 +' &1))) _ _,
+  from L_abel_structure_of_add_comm_group α, from ⟨0⟩,
+  from add_comm_group_is_abelian_group, by refl,
+  from T_ab_proves_x_y_y
 end
 
 end
